atomic_deduction.v
@@ -7,11 +7,18 @@ Reserved Notation "A ⊢A p" (at level 70).
 
 Section atomic.
   Variable form : Type.
-  Variable retract : retract (form_atomic) form.
 
+  Variable retract : retract (form_atomic) form.
   Variable retract_implicative : included form_implicative form.
 
   Variable translate : form -> form.
   Definition translate_atomic (p : form_atomic) : form := ¬¬(inj p).
+  Notation "« p »" := (translate p).
+
+  Variable subst_form : (fin -> term) -> form -> form.
+  Variable translation_subst : forall sigma q, «subst_form sigma q» = subst_form sigma «q».
+  Lemma translation_subst_atm sigma q : «subst_form sigma (inj q)» = subst_form sigma «inj q».
+  Proof. destruct q; repeat now rewrite translation_subst.
+  Defined.
 
 End atomic.
