universal_deduction.v
@@ -25,57 +25,44 @@ Section universals.
     | ndUE p t : A ⊢ ∀ p -> A ⊢U subst_form (scons t (var_term)) p
   where "A ⊢U p" := (nd_univ A p).
 
-(*   Variable agree : forall A p, A ⊢U p -> A ⊢ p.
- *)
   Variable weakening : forall A B p, A ⊢ p -> incl A B -> B ⊢ p.
   Lemma weakening_univ A B p : A ⊢U p -> incl A B -> B ⊢U p.
   Proof. intro. revert B. destruct H; intros B Hinc; [ apply ndUI | now apply ndUE, (weakening A) ].
     -apply (weakening (up_ctx A) (up_ctx B)); [ assumption | unfold up_ctx ]. now apply incl_map.
   Defined.
 
-
-(*   Variable retract_implicative : included form_implicative form.
- *)
   Variable translate : form -> form.
   Definition translate_univ (p : form_universal form) : _ := match p with
     | All _ q => All _ (translate q)
   end.
 
-  Variable translation_inj : forall p, translate (inj p) = inj (translate_univ p).
-  Variable translation_subst : forall q sigma, translate (subst_form sigma q) = subst_form sigma (translate q).
-  Variable translation_int : forall A p, A ⊢ p -> (map translate A) ⊢ (translate p).
-
-  Lemma translation_map A: up_ctx (map translate A) = map translate (up_ctx A).
-  Proof. unfold up_ctx. repeat rewrite map_map. apply map_ext. intro p. symmetry. apply translation_subst.
-  Qed.
-
-  Lemma translation_int_univ A p : A ⊢U p -> (map translate A) ⊢U (translate p).
-  Proof. destruct 1.
-    -rewrite translation_inj. cbn. apply ndUI. rewrite translation_map. now apply translation_int.
-    -rewrite translation_subst. apply ndUE. pose (translation_inj (All _ p)). cbn in e. rewrite <- e.
-     now apply translation_int.
-  Defined.
 
 End universals.
 
 Notation "A ⊢U p" := (nd_univ A p) (at level 70).
 
 Section translation.
+Require Import classical_deduction.
 
   Variable form : Type.
   Variable subst_form : (fin -> term) -> form -> form.
   Variable retract_univ : retract (form_universal form) form.
-(*   Variable retract_implicative : included form_implicative form.
- *)
-  Notation "A ⊢[ nd ] p" := (@nd_univ form _ subst_form nd A p) (at level 70).
   Variable translate : form -> form.
+
+  Notation "A ⊢[ nd ] p" := (@nd_univ form _ subst_form nd A p) (at level 70).
   Notation "« p »" := (translate p).
   Notation "«/ A »" := (map translate A).
 
   Variable translation_inj : forall p, «inj p» = inj (translate_univ _ translate p).
+  Variable translation_subst : forall sigma q, «subst_form sigma q» = subst_form sigma «q».
 
-  Require Import classical_deduction.
-  Variable retract_implicative : included form_implicative form.
+  Lemma translation_subst_univ sigma q: «subst_form sigma (inj q)» = subst_form sigma «inj q».
+  Proof. destruct q. rewrite translation_subst. rewrite translation_inj. auto.
+  Defined.
+
+  Lemma translation_map A: up_ctx form subst_form (map translate A) = map translate (up_ctx form subst_form A).
+  Proof. unfold up_ctx. repeat rewrite map_map. apply map_ext. intro p. symmetry. apply translation_subst.
+  Qed.
 
   Variable nd : list form -> form -> Prop.
   Variable cnd : list form -> form -> Prop.
@@ -85,13 +72,10 @@ Section translation.
   Proof. destruct 1; [ now apply ndUI, embed | now apply ndUE, embed ].
   Defined.
 
-
-  Variable translation_subst : forall q sigma, translate (subst_form sigma q) = subst_form sigma (translate q).
-
   Variable translation : forall A p, cnd A p -> nd «/A» «p».
   Lemma translation_univ A p: A ⊢[cnd] p -> «/A» ⊢[nd] «p».
   Proof. destruct 1.
-    +rewrite translation_inj. cbn. apply ndUI. rewrite translation_map. now apply translation. exact translation_subst.
+    +rewrite translation_inj. cbn. apply ndUI. rewrite translation_map. now apply translation.
     +rewrite translation_subst. apply ndUE. { pose (translation_inj (All _ p)). cbn in e. rewrite <- e. now apply translation. }
   Defined.
 End translation.
